move SourceLifted proofs into a separate file

src/SourceLifted.v
@@ -17,8 +17,6 @@ Definition type_eq_dec (t1 t2 : type) : {t1 = t2} + {t1 <> t2}.
   decide equality; auto using type_name_eq_dec.
 Defined.
 
-
-
 Inductive constr_type : constr_name -> list type -> type_name -> Type :=
 | CTO            : constr_type CO         []                          Tnat
 | CTS            : constr_type CS         [ADT Tnat]                  Tnat
@@ -85,89 +83,18 @@ End expr.
 Implicit Arguments value.
 Implicit Arguments expr.
 
+Inductive is_value {G L ty} : expr G L ty -> Prop :=
+| IsValue : forall v, is_value (Value v).
+
 Definition body_expr G fn_sig :=
     let '(arg_ty, free_tys, ret_ty) := fn_sig in
     expr G (arg_ty :: free_tys) ret_ty.
 
 
-Definition value_rect_mut_comb G
-        (P : forall {ty}, value G ty -> Type)
-        (Pl : forall {tys}, hlist (value G) tys -> Type)
-    (HVConstr : forall {ty ctor arg_tys} (ct : constr_type ctor arg_tys ty) args,
-        Pl args -> P (VConstr ct args))
-    (HVClose : forall {arg_ty free_tys ret_ty} (mb : member (arg_ty, free_tys, ret_ty) G) free,
-        Pl free -> P (VClose mb free))
-    (Hhnil : Pl hnil)
-    (Hhcons : forall {ty tys} (v : value G ty) (vs : hlist (value G) tys),
-        P v -> Pl vs -> Pl (hcons v vs)) :
-    (forall {ty} (v : value G ty), P v) *
-    (forall {tys} (v : hlist (value G) tys), Pl v) :=
-    let fix go {ty} (v : value G ty) :=
-        let fix go_hlist {tys} (vs : hlist (value G) tys) :=
-            match vs as vs_ return Pl vs_ with
-            | hnil => Hhnil
-            | hcons v vs => Hhcons v vs (go v) (go_hlist vs)
-            end in
-        match v as v_ return P v_ with
-        | VConstr ct args => HVConstr ct args (go_hlist args)
-        | VClose mb free => HVClose mb free (go_hlist free)
-        end in
-    let fix go_hlist {tys} (vs : hlist (value G) tys) :=
-        match vs as vs_ return Pl vs_ with
-        | hnil => Hhnil
-        | hcons v vs => Hhcons v vs (go v) (go_hlist vs)
-        end in
-    (@go, @go_hlist).
+(* weakening: convert an expr in `G` into an expr in an extension of `G` *)
 
-Definition value_rect_mut G P Pl HVConstr HVClose Hhnil Hhcons :=
-    fst (value_rect_mut_comb G P Pl HVConstr HVClose Hhnil Hhcons).
-
-
-Definition expr_rect_mut_comb G L
-        (P : forall {ty}, expr G L ty -> Type)
-        (Pl : forall {tys}, hlist (expr G L) tys -> Type)
-    (HValue : forall {ty} (v : value G ty), P (Value v))
-    (HVar : forall {ty} (mb : member ty L), P (Var mb))
-    (HApp : forall {ty1 ty2} (f : expr G L (Arrow ty1 ty2)) (a : expr G L ty1),
-        P f -> P a -> P (App f a))
-    (HConstr : forall {ty ctor arg_tys} (ct : constr_type ctor arg_tys ty) args,
-        Pl args -> P (Constr ct args))
-    (HClose : forall {arg_ty free_tys ret_ty} (mb : member (arg_ty, free_tys, ret_ty) G) free,
-        Pl free -> P (Close mb free))
-    (HElim : forall {case_tys target_tyn ty} (e : elim case_tys (ADT target_tyn) ty) cases target,
-        Pl cases -> P target -> P (Elim e cases target))
-    (Hhnil : Pl hnil)
-    (Hhcons : forall {ty tys} (e : expr G L ty) (es : hlist (expr G L) tys),
-        P e -> Pl es -> Pl (hcons e es)) :
-    (forall {ty} (e : expr G L ty), P e) *
-    (forall {tys} (e : hlist (expr G L) tys), Pl e) :=
-    let fix go {ty} (e : expr G L ty) :=
-        let fix go_hlist {tys} (es : hlist (expr G L) tys) :=
-            match es as es_ return Pl es_ with
-            | hnil => Hhnil
-            | hcons e es => Hhcons e es (go e) (go_hlist es)
-            end in
-        match e as e_ return P e_ with
-        | Value v => HValue v
-        | Var mb => HVar mb
-        | App f a => HApp f a (go f) (go a)
-        | Constr ct args => HConstr ct args (go_hlist args)
-        | Close mb free => HClose mb free (go_hlist free)
-        | Elim e cases target => HElim e cases target (go_hlist cases) (go target)
-        end in
-    let fix go_hlist {tys} (es : hlist (expr G L) tys) :=
-        match es as es_ return Pl es_ with
-        | hnil => Hhnil
-        | hcons e es => Hhcons e es (go e) (go_hlist es)
-        end in
-    (@go, @go_hlist).
-
-Definition expr_rect_mut G L P Pl HValue HVar HApp HConstr HClose HElim Hhnil Hhcons :=
-    fst (expr_rect_mut_comb G L P Pl HValue HVar HApp HConstr HClose HElim Hhnil Hhcons).
-
-
-
-Definition weaken_value {G} fn_sig : forall {ty}, value G ty -> value (fn_sig :: G) ty :=
+Definition weaken_value {G} fn_sig :
+        forall {ty}, value G ty -> value (fn_sig :: G) ty :=
     let fix go {ty} (v : value G ty) : value (fn_sig :: G) ty :=
         let fix go_hlist {tys} (vs : hlist (value G) tys) : hlist (value (fn_sig :: G)) tys :=
             match vs with
@@ -188,7 +115,8 @@ Definition weaken_value_hlist {G} fn_sig :
         | hcons v vs => hcons (go _ v) (go_hlist vs)
         end in @go_hlist.
 
-Definition weaken {G L} fn_sig : forall {ty}, expr G L ty -> expr (fn_sig :: G) L ty :=
+Definition weaken_expr {G L} fn_sig :
+        forall {ty}, expr G L ty -> expr (fn_sig :: G) L ty :=
     let fix go {ty} (e : expr G L ty) : expr (fn_sig :: G) L ty :=
         let fix go_hlist {tys} (es : hlist (expr G L) tys) : hlist (expr (fn_sig :: G) L) tys :=
             match es with
@@ -205,9 +133,9 @@ Definition weaken {G L} fn_sig : forall {ty}, expr G L ty -> expr (fn_sig :: G) 
         end
     in @go.
 
-Definition weaken_hlist {G L} fn_sig :
+Definition weaken_expr_hlist {G L} fn_sig :
         forall {tys}, hlist (expr G L) tys -> hlist (expr (fn_sig :: G) L) tys :=
-    let go := @weaken G L fn_sig in
+    let go := @weaken_expr G L fn_sig in
     let fix go_hlist {tys} (es : hlist (expr G L) tys) : hlist (expr (fn_sig :: G) L) tys :=
         match es with
         | hnil => hnil
@@ -218,13 +146,13 @@ Definition weaken_body {G} fn_sig :
         forall {sig}, body_expr G sig -> body_expr (fn_sig :: G) sig :=
     fun sig =>
         match sig as sig_ return body_expr _ sig_ -> body_expr _ sig_ with
-        | (arg_ty, free_tys, fn_ty) => fun e => weaken fn_sig e
+        | (arg_ty, free_tys, fn_ty) => fun e => weaken_expr fn_sig e
         end.
 
 
 
-Inductive is_value {G L ty} : expr G L ty -> Prop :=
-| IsValue : forall v, is_value (Value v).
+(* (static) global environments.  Similar to an hlist, but each value can refer
+   to the tail that comes after it. *)
 
 Inductive genv : list (type * list type * type) -> Set :=
 | GenvNil : genv []
@@ -233,107 +161,13 @@ Inductive genv : list (type * list type * type) -> Set :=
         genv rest ->
         genv (fn_sig :: rest).
 
-
-Lemma hlist_member_rect A (B : A -> Type) (ix : A)
-        (P : forall ixs, hlist B ixs -> member ix ixs -> Type)
-    (HHere : forall ixs val vals,
-        P (ix :: ixs) (hcons val vals) Here)
-    (HThere : forall ix' ixs val vals mb
-        (IHmb : P ixs vals mb),
-        P (ix' :: ixs) (hcons val vals) (There mb))
-    : forall ixs vals mb, P ixs vals mb.
-induction vals; intros.
-
-- exfalso.
-  refine (
-    match mb in member _ [] with
-    | Here => idProp
-    | There mb' => idProp
-    end).
-
-- rename a into ix'. rename b into val. rename l into ixs.
-  refine (
-    match mb as mb_ in member _ (ix'_ :: ixs_)
-        return (
-            forall (val_ : B ix'_) (vals_ : hlist B ixs_)
-                (IHvals_ : forall mb, P ixs_ vals_ mb),
-            P (ix'_ :: ixs_) (hcons val_ vals_) mb_) with
-    | Here => _
-    | There mb' => _
-    end val vals IHvals); intros.
-  + eapply HHere.
-  + eapply HThere. eapply IHvals_.
-Defined.
-
-Lemma hlist_member_ind A (B : A -> Type) (ix : A)
-        (P : forall ixs, hlist B ixs -> member ix ixs -> Prop)
-    (HHere : forall ixs val vals,
-        P (ix :: ixs) (hcons val vals) Here)
-    (HThere : forall ix' ixs val vals mb
-        (IHmb : P ixs vals mb),
-        P (ix' :: ixs) (hcons val vals) (There mb))
-    : forall ixs vals mb, P ixs vals mb.
-apply hlist_member_rect; assumption.
-Qed.
-
-Lemma genv_member_rect ix
-        (P : forall ixs, genv ixs -> member ix ixs -> Type)
-    (HHere : forall ixs val vals,
-        P (ix :: ixs) (GenvCons val vals) Here)
-    (HThere : forall ix' ixs val vals mb
-        (IHmb : P ixs vals mb),
-        P (ix' :: ixs) (GenvCons val vals) (There mb))
-    : forall G g mb, P G g mb.
-induction g using genv_rect; intros.
-
-- exfalso.
-  refine (
-    match mb in member _ [] with
-    | Here => idProp
-    | There mb' => idProp
-    end).
-
-- rename fn_sig into ix'. rename rest into ixs.
-  rename b into val. rename g into vals.
-  rename IHg into IHvals.
-
-  refine (
-    match mb as mb_ in member _ (ix'_ :: ixs_)
-        return (
-            forall (val_ : body_expr ixs_ ix'_) (vals_ : genv ixs_)
-                (IHvals_ : forall mb, P ixs_ vals_ mb),
-            P (ix'_ :: ixs_) (GenvCons val_ vals_) mb_) with
-    | Here => _
-    | There mb' => _
-    end val vals IHvals); intros.
-
-  + eapply HHere.
-  + eapply HThere. eapply IHvals_.
-Defined.
-
-Print genv_member_rect.
-
-Lemma genv_member_ind ix
-        (P : forall ixs, genv ixs -> member ix ixs -> Prop)
-    (HHere : forall ixs val vals,
-        P (ix :: ixs) (GenvCons val vals) Here)
-    (HThere : forall ix' ixs val vals mb
-        (IHmb : P ixs vals mb),
-        P (ix' :: ixs) (GenvCons val vals) (There mb))
-    : forall G g mb, P G g mb.
-apply genv_member_rect; assumption.
-Qed.
-
-
-
-
-
 Definition mtail {A x} l : @member A x l -> list A.
 induction 1.
 - exact l.
 - exact IHX.
 Defined.
 
+(* retrieve a value from a genv *)
 Fixpoint gget {G} (g : genv G) {fn_sig} (mb : member fn_sig G) {struct g} :
         body_expr (mtail G mb) fn_sig * genv (mtail G mb).
 rename G into ixs. rename g into vals.
@@ -373,6 +207,7 @@ refine (
 - simpl. eapply gget.
 Defined.
 
+(* retrieve a value from a genv, and weaken it to be valid in the whole genv *)
 Fixpoint gget_weaken {G} (g : genv G) {fn_sig} (mb : member fn_sig G) {struct g} :
         body_expr G fn_sig.
 rename G into ixs. rename g into vals.
@@ -414,7 +249,7 @@ Defined.
 
 
 
-
+(* denotation functions *)
 
 Fixpoint type_denote (ty : type) : Type :=
   match ty with
@@ -457,8 +292,188 @@ Definition elim_denote {case_tys target_ty ty} (e : elim case_tys target_ty ty) 
                                                  (hhead (htail (htail cases))) target
   end.
 
+Definition value_denote
+        {G} (g : hlist func_type_denote G) :
+        forall {ty}, value G ty -> type_denote ty :=
+    let fix go {ty} (v : value G ty) : type_denote ty :=
+        let fix go_hlist {tys} (vs : hlist (value G) tys) : hlist type_denote tys :=
+            match vs with
+            | hnil => hnil
+            | hcons v vs => hcons (go v) (go_hlist vs)
+            end in
+        match v with
+        | VConstr ct args => constr_denote ct (go_hlist args)
+        | VClose mb free =>
+                let func := hget g mb in
+                let free' := go_hlist free in
+                fun x => func free' x
+        end in @go.
+
+Definition value_hlist_denote
+        {G} (g : hlist func_type_denote G) :
+        forall {tys}, hlist (value G) tys -> hlist type_denote tys :=
+    let go := @value_denote G g in
+    let fix go_hlist {tys} (vs : hlist (value G) tys) : hlist type_denote tys :=
+        match vs with
+        | hnil => hnil
+        | hcons v vs => hcons (go _ v) (go_hlist vs)
+        end in @go_hlist.
+
+Definition expr_denote {G L} (g : hlist func_type_denote G) (l : hlist type_denote L) :
+        forall {ty}, expr G L ty -> type_denote ty :=
+    let fix go {ty} (e : expr G L ty) {struct e} : type_denote ty :=
+        let fix go_hlist {tys} (es : hlist (expr G L) tys) {struct es} : hlist type_denote tys :=
+            match es with
+            | hnil => hnil
+            | hcons e es => hcons (go e) (go_hlist es)
+            end in
+        match e with
+        | Value v => value_denote g v
+        | Var mb => hget l mb
+        | App f a => (go f) (go a)
+        | Constr ct args => constr_denote ct (go_hlist args)
+        | Close mb free =>
+            let func := hget g mb in
+            let free' := go_hlist free in
+            fun x => func free' x
+        | Elim e cases target => elim_denote e (go_hlist cases) (go target)
+        end in @go.
+
+Definition expr_hlist_denote {G L} (g : hlist func_type_denote G) (l : hlist type_denote L) :
+        forall {tys}, hlist (expr G L) tys -> hlist type_denote tys :=
+    let go := @expr_denote G L g l in
+    let fix go_hlist {tys} (vs : hlist (expr G L) tys) : hlist type_denote tys :=
+        match vs with
+        | hnil => hnil
+        | hcons v vs => hcons (go _ v) (go_hlist vs)
+        end in @go_hlist.
+
+Definition body_expr_denote
+        {G} (g : hlist func_type_denote G)
+        {fn_sig} (e : body_expr G fn_sig) :
+        func_type_denote fn_sig :=
+    match fn_sig as fn_sig_ return body_expr G fn_sig_ -> func_type_denote fn_sig_ with
+    | (arg_ty, free_tys, ret_ty) => fun e =>
+            fun l x => expr_denote g (hcons x l) e
+    end e.
+
+Definition genv_denote {G} (g : genv G) : hlist func_type_denote G :=
+    let fix go {G} (g : genv G) : hlist func_type_denote G :=
+        match g with
+        | GenvNil => hnil
+        | GenvCons e g' =>
+                let g'_den := go g' in
+                hcons (body_expr_denote g'_den e) g'_den
+        end in go g.
 
 
+(* program states *)
+
+(* `cont G rty ty`: a continuation, valid in global environment `G`, that
+   requires a value of type `ty`, and eventually proceeds to a `Stop` state
+   containing a result value of type `rty` (assuming termination). *)
+Inductive cont {G} {rty : type} : type -> Set :=
+| KAppL {L ty1 ty2}
+        (e2 : expr G L ty1)
+        (l : hlist (value G) L)
+        (k : cont ty2)
+        : cont (Arrow ty1 ty2)
+| KAppR {L ty1 ty2}
+        (e1 : expr G L (Arrow ty1 ty2))
+        (l : hlist (value G) L)
+        (k : cont ty2)
+        : cont ty1
+| KConstr {L vtys ety etys ctor ty}
+        (ct : constr_type ctor (vtys ++ [ety] ++ etys) ty)
+        (vs : hlist (expr G L) vtys)
+        (es : hlist (expr G L) etys)
+        (l : hlist (value G) L)
+        (k : cont (ADT ty))
+        : cont ety
+| KClose {L vtys ety etys arg_ty ret_ty}
+        (mb : member (arg_ty, vtys ++ [ety] ++ etys, ret_ty) G)
+        (vs : hlist (expr G L) vtys)
+        (es : hlist (expr G L) etys)
+        (l : hlist (value G) L)
+        (k : cont (Arrow arg_ty ret_ty))
+        : cont ety
+| KElim {L case_tys target_tyn ty}
+        (e : elim case_tys (ADT target_tyn) ty)
+        (cases : hlist (expr G L) case_tys)
+        (l : hlist (value G) L)
+        (k : cont ty)
+        : cont (ADT target_tyn)
+| KStop : cont rty
+.
+Implicit Arguments cont [].
+
+(* `state G rty`: a state, valid in global environment `G`, that will
+   eventually proceed to a `Stop` state containing a result value of type `rty`
+   (assuming termination). *)
+Inductive state {G rty} :=
+| Run {L ty}
+        (e : expr G L ty)
+        (l : hlist (value G) L)
+        (k : cont G rty ty)
+| Stop (v : value G rty).
+Implicit Arguments state [].
+
+(* denotation of program states *)
+
+Definition cont_denote {G rty ty} (g : hlist func_type_denote G) (k : cont G rty ty) :
+        type_denote ty -> type_denote rty :=
+    let locals_denote {tys} (l : hlist _ tys) := value_hlist_denote g l in
+    let fix go {ty} (k : cont G rty ty) :=
+        match k in cont _ _ ty_ return type_denote ty_ -> type_denote rty with
+        | KAppL e2 l k => fun x => go k (x (expr_denote g (locals_denote l) e2))
+        | KAppR e1 l k => fun x => go k ((expr_denote g (locals_denote l) e1) x)
+        | KConstr ct vs es l k => fun x =>
+                let l' := locals_denote l in
+                let vs' := expr_hlist_denote g l' vs in
+                let es' := expr_hlist_denote g l' es in
+                go k (constr_denote ct (happ vs' (hcons x es')))
+        | KClose mb vs es l k => fun x =>
+                let l' := locals_denote l in
+                let vs' := expr_hlist_denote g l' vs in
+                let es' := expr_hlist_denote g l' es in
+                let func := hget g mb in
+                go k (fun arg => func (happ vs' (hcons x es')) arg)
+        | KElim e cases l k => fun x =>
+                let l' := locals_denote l in
+                let cases' := expr_hlist_denote g l' cases in
+                go k (elim_denote e cases' x)
+        | KStop => fun x => x
+        end in go k.
+
+Definition state_denote {G rty} (g : hlist func_type_denote G) (s : state G rty) :
+        type_denote rty :=
+    match s with
+    | Run e l k =>
+            let e' := expr_denote g (value_hlist_denote g l) e in
+            let k' := cont_denote g k in
+            k' e'
+    | Stop v => value_denote g v
+    end.
+
+
+(* operational semantics - step relation *)
+
+(* helper function for proceeding into a continuation *)
+Definition run_cont {G rty ty} (k : cont G rty ty) : value G ty -> state G rty :=
+    match k in cont _ _ ty_ return value G ty_ -> state G rty with
+    | KAppL e2 l k => fun v => Run (App (Value v) e2) l k
+    | KAppR e1 l k => fun v => Run (App e1 (Value v)) l k
+    | KConstr ct vs es l k =>
+            fun v => Run (Constr ct (happ vs (hcons (Value v) es))) l k
+    | KClose mb vs es l k =>
+            fun v => Run (Close mb (happ vs (hcons (Value v) es))) l k
+    | KElim e cases l k =>
+            fun v => Run (Elim e cases (Value v)) l k
+    | KStop => fun v => Stop v
+    end.
+
+(* helper function for the "eliminate" step.  Analogous to `unroll_elim` in
+   later passes. *)
 Section run_elim.
 Local Notation "f $ a" := (App f a) (at level 50, left associativity, only parsing).
 
@@ -483,6 +498,8 @@ refine (
     end e).
 clear e0 target target_tyn0.
 
+(* note: if you add any new cases here, you must also add cases to
+   run_elim_denote in SourceLiftedProofs.v *)
 refine (
     match e in elim case_tys_ (ADT target_tyn_) ret_ty_
         return forall
@@ -595,110 +612,92 @@ Defined.
 
 End run_elim.
 
+(* the actual step relation *)
+Inductive sstep {G rty} (g : genv G) : state G rty -> state G rty -> Prop :=
+| SValue : forall {L ty} v (l : hlist (value G) L) (k : cont G rty ty),
+        sstep g (Run (Value v) l k)
+                (run_cont k v)
 
-Definition value_denote
-        {G} (g : hlist func_type_denote G) :
-        forall {ty}, value G ty -> type_denote ty :=
-    let fix go {ty} (v : value G ty) : type_denote ty :=
-        let fix go_hlist {tys} (vs : hlist (value G) tys) : hlist type_denote tys :=
-            match vs with
-            | hnil => hnil
-            | hcons v vs => hcons (go v) (go_hlist vs)
-            end in
-        match v with
-        | VConstr ct args => constr_denote ct (go_hlist args)
-        | VClose mb free =>
-                let func := hget g mb in
-                let free' := go_hlist free in
-                fun x => func free' x
-        end in @go.
+| SVar : forall {L ty} mb (l : hlist (value G) L) (k : cont G rty ty),
+        sstep g (Run (Var mb) l k)
+        (* TODO: simplify *)
+                (Run (Value (hget l mb)) l k)
 
-Definition value_hlist_denote
-        {G} (g : hlist func_type_denote G) :
-        forall {tys}, hlist (value G) tys -> hlist type_denote tys :=
-    let go := @value_denote G g in
-    let fix go_hlist {tys} (vs : hlist (value G) tys) : hlist type_denote tys :=
-        match vs with
-        | hnil => hnil
-        | hcons v vs => hcons (go _ v) (go_hlist vs)
-        end in @go_hlist.
+| SAppL : forall {L ty1 ty2} (e1 : expr G L (Arrow ty1 ty2)) (e2 : expr G L ty1) l k,
+        ~ is_value e1 ->
+        sstep g (Run (App e1 e2) l k)
+                (Run e1 l (KAppL e2 l k))
 
-Definition expr_denote {G L} (g : hlist func_type_denote G) (l : hlist type_denote L) :
-        forall {ty}, expr G L ty -> type_denote ty :=
-    let fix go {ty} (e : expr G L ty) {struct e} : type_denote ty :=
-        let fix go_hlist {tys} (es : hlist (expr G L) tys) {struct es} : hlist type_denote tys :=
-            match es with
-            | hnil => hnil
-            | hcons e es => hcons (go e) (go_hlist es)
-            end in
-        match e with
-        | Value v => value_denote g v
-        | Var mb => hget l mb
-        | App f a => (go f) (go a)
-        | Constr ct args => constr_denote ct (go_hlist args)
-        | Close mb free =>
-            let func := hget g mb in
-            let free' := go_hlist free in
-            fun x => func free' x
-        | Elim e cases target => elim_denote e (go_hlist cases) (go target)
-        end in @go.
+| SAppR : forall {L ty1 ty2} (e1 : expr G L (Arrow ty1 ty2)) (e2 : expr G L ty1) l k,
+        is_value e1 ->
+        ~ is_value e2 ->
+        sstep g (Run (App e1 e2) l k)
+                (Run e2 l (KAppR e1 l k))
 
-Definition expr_hlist_denote {G L} (g : hlist func_type_denote G) (l : hlist type_denote L) :
-        forall {tys}, hlist (expr G L) tys -> hlist type_denote tys :=
-    let go := @expr_denote G L g l in
-    let fix go_hlist {tys} (vs : hlist (expr G L) tys) : hlist type_denote tys :=
-        match vs with
-        | hnil => hnil
-        | hcons v vs => hcons (go _ v) (go_hlist vs)
-        end in @go_hlist.
+| SMakeCall : forall {L arg_ty free_tys ret_ty}
+            (mb : member (arg_ty, free_tys, ret_ty) G) free arg
+            (l : hlist _ L) k,
+        sstep g (Run (App (Value (VClose mb free)) (Value arg)) l k)
+                (Run (gget_weaken g mb) (hcons arg free) k)
 
-Definition body_expr_denote' {G arg_ty free_tys ret_ty}
-        (g : hlist func_type_denote G) (e : body_expr G (arg_ty, free_tys, ret_ty)) :
-        func_type_denote (arg_ty, free_tys, ret_ty) :=
-    fun l x => expr_denote g (hcons x l) e.
+| SConstrStep : forall {L vtys ety etys ctor ty}
+            (ct : constr_type ctor (vtys ++ [ety] ++ etys) ty)
+            (vs : hlist (expr G L) vtys)
+            (e : expr G L ety)
+            (es : hlist (expr G L) etys)
+            (l : hlist _ L) k,
+        HForall (@is_value G L) vs ->
+        ~ is_value e ->
+        sstep g (Run (Constr ct (happ vs (hcons e es))) l k)
+                (Run e l (KConstr ct vs es l k))
+| SConstrDone : forall {L vtys ctor ty}
+            (ct : constr_type ctor vtys ty)
+            (vs : hlist (value G) vtys)
+            (l : hlist _ L) k,
+        let es := hmap (@Value G L) vs in
+        sstep g (Run (Constr ct es) l k)
+                (Run (Value (VConstr ct vs)) l k)
 
-Definition body_expr_denote
-        {G} (g : hlist func_type_denote G)
-        {fn_sig} (e : body_expr G fn_sig) :
-        func_type_denote fn_sig :=
-    match fn_sig as fn_sig_ return body_expr G fn_sig_ -> func_type_denote fn_sig_ with
-    | (arg_ty, free_tys, ret_ty) => fun e =>
-            fun l x => expr_denote g (hcons x l) e
-    end e.
+| SCloseStep : forall {L vtys ety etys arg_ty ret_ty}
+            (mb : member (arg_ty, vtys ++ [ety] ++ etys, ret_ty) G)
+            (vs : hlist (expr G L) vtys)
+            (e : expr G L ety)
+            (es : hlist (expr G L) etys)
+            (l : hlist _ L) k,
+        HForall (@is_value G L) vs ->
+        ~ is_value e ->
+        sstep g (Run (Close mb (happ vs (hcons e es))) l k)
+                (Run e l (KClose mb vs es l k))
+| SCloseDone : forall {L vtys arg_ty ret_ty}
+            (mb : member (arg_ty, vtys, ret_ty) G)
+            (vs : hlist (value G) vtys)
+            (l : hlist _ L) k,
+        let es := hmap (@Value G L) vs in
+        sstep g (Run (Close mb es) l k)
+                (Run (Value (VClose mb vs)) l k)
 
-Definition genv_denote {G} (g : genv G) : hlist func_type_denote G :=
-    let fix go {G} (g : genv G) : hlist func_type_denote G :=
-        match g with
-        | GenvNil => hnil
-        | GenvCons e g' =>
-                let g'_den := go g' in
-                hcons (body_expr_denote g'_den e) g'_den
-        end in go g.
+| SElimTarget : forall {L case_tys target_tyn ty}
+            (e : elim case_tys (ADT target_tyn) ty)
+            (cases : hlist (expr G L) case_tys)
+            (target : expr G L (ADT target_tyn))
+            (l : hlist _ L) k,
+        ~ is_value target ->
+        sstep g (Run (Elim e cases target) l k)
+                (Run target l (KElim e cases l k))
 
-Lemma genv_denote_gget' : forall {G} g {fn_sig} (mb : member fn_sig G),
-    hget (genv_denote g) mb =
-    (let '(e, g') := gget g mb in
-        body_expr_denote (genv_denote g') e).
-intros.
-eapply genv_member_ind with (g := g) (mb := mb); intros.
-- simpl. reflexivity.
-- simpl. exact IHmb.
-Qed.
-
-Lemma genv_denote_gget : forall
-        {G} (g : genv G)
-        {arg_ty free_tys ret_ty} (mb : member (arg_ty, free_tys, ret_ty) G)
-        l x,
-    hget (genv_denote g) mb l x =
-    (let '(e, g') := gget g mb in
-        expr_denote (genv_denote g') (hcons x l) e).
-intros.
-eapply genv_member_ind with (g := g) (mb := mb); intros; simpl.
-- reflexivity.
-- exact IHmb.
-Qed.
+| SEliminate : forall {L case_tys target_tyn ty}
+            (e : elim case_tys (ADT target_tyn) ty)
+            (cases : hlist (expr G L) case_tys)
+            (target : value G (ADT target_tyn))
+            (l : hlist _ L) k,
+        sstep g (Run (Elim e cases (Value target)) l k)
+                (Run (run_elim e cases target) l k)
+.
 
 
+
+
+(* example program *)
 
 Section add.
 
@@ -723,8 +722,6 @@ Qed.
 
 Local Notation "t1 '~>' t2" := (Arrow t1 t2) (right associativity, at level 100, only parsing).
 Local Notation "'N'" := (ADT Tnat) (only parsing).
-
-Print add_lifted.
 
 Definition add_G' :=
     [ (* Hzero *) (N, [], N)
@@ -800,10 +797,10 @@ Definition add_genv : genv add_G :=
     (GenvCons add_Hzero
     (GenvNil))))))).
 
-Eval compute -[type_denote] in genv_denote add_genv.
+(* Eval compute -[type_denote] in genv_denote add_genv. *)
 
 Definition add_denoted := hhead (genv_denote add_genv) hnil.
-Eval compute in add_denoted 1 2.
+(* Eval compute in add_denoted 1 2. *)
 
 Lemma add_denoted_eq : add_denoted = add_elim.
 reflexivity.
@@ -813,563 +810,6 @@ Definition zero : value add_G N := VConstr CTO hnil.
 Definition one : value add_G N := VConstr CTS (hcons zero hnil).
 Definition two : value add_G N := VConstr CTS (hcons one hnil).
 Definition three : value add_G N := VConstr CTS (hcons two hnil).
-Eval compute in value_denote (genv_denote add_genv) three.
+(* Eval compute in value_denote (genv_denote add_genv) three. *)
 
 End add.
-
-
-
-
-Lemma weaken_value_denote : forall {G ty} fn_sig func g (v : value G ty),
-    value_denote g v = value_denote (hcons func g) (weaken_value fn_sig v).
-intros until v.
-induction v using value_rect_mut with
-    (Pl := fun tys vs =>
-        value_hlist_denote g vs =
-        value_hlist_denote _ (weaken_value_hlist fn_sig vs));
-simpl;
-fold (@value_hlist_denote _ g);
-fold (@value_hlist_denote _ (hcons func g));
-fold (@weaken_value_hlist G fn_sig).
-
-- f_equal. exact IHv.
-- rewrite <- IHv. reflexivity.
-
-- reflexivity.
-- erewrite <- IHv, <- IHv0. reflexivity.
-
-Qed.
-
-Lemma weaken_expr_denote : forall {G L ty} fn_sig func g l (e : expr G L ty),
-    expr_denote g l e = expr_denote (hcons func g) l (weaken fn_sig e).
-intros until e.
-induction e using expr_rect_mut with
-    (Pl := fun tys es =>
-        expr_hlist_denote g l es =
-        expr_hlist_denote _ _ (weaken_hlist fn_sig es));
-simpl;
-fold (@expr_hlist_denote _ _ g l);
-fold (@expr_hlist_denote _ _ (hcons func g) l);
-fold (@weaken_hlist G L fn_sig).
-
-- eapply weaken_value_denote.
-- reflexivity.
-- rewrite <- IHe1, <- IHe2. reflexivity.
-- rewrite <- IHe. reflexivity.
-- rewrite <- IHe. reflexivity.
-- rewrite <- IHe, <- IHe0. reflexivity.
-
-- reflexivity.
-- erewrite <- IHe, <- IHe0. reflexivity.
-
-Qed.
-
-Lemma weaken_body_denote : forall {G sig} fn_sig func g (e : body_expr G sig),
-    body_expr_denote g e = body_expr_denote (hcons func g) (weaken_body fn_sig e).
-intros.
-destruct sig as [[? ?] ?]. simpl in *.
-do 2 (eapply functional_extensionality; intro).
-eapply weaken_expr_denote.
-Qed.
-
-Lemma gget_gget_weaken' : forall {G} g {fn_sig} (mb : member fn_sig G),
-    body_expr_denote (genv_denote g) (gget_weaken g mb) =
-    let '(e, g') := gget g mb in
-        body_expr_denote (genv_denote g') e.
-intros.
-eapply genv_member_ind with (g := g) (mb := mb); intros; simpl.
-- rewrite <- weaken_body_denote. reflexivity.
-- rewrite <- weaken_body_denote. exact IHmb.
-Qed.
-
-Lemma gget_gget_weaken : forall
-        {G} (g : genv G)
-        {arg_ty free_tys ret_ty} (mb : member (arg_ty, free_tys, ret_ty) G)
-        l,
-    expr_denote (genv_denote g) l (gget_weaken g mb) =
-    let '(e, g') := gget g mb in
-        expr_denote (genv_denote g') l e.
-intros.
-eapply genv_member_ind with (g := g) (mb := mb); intros; simpl.
-- rewrite <- weaken_expr_denote. reflexivity.
-- rewrite <- weaken_expr_denote. exact IHmb.
-Qed.
-
-
-
-
-Lemma hmap_app : forall {A B C} {l l' : list A} (f : forall a, B a -> C a)
-        (h : hlist B l) (h' : hlist B l'),
-    hmap f (happ h h') = happ (hmap f h) (hmap f h').
-induction h; intros; simpl in *.
-- reflexivity.
-- rewrite IHh. reflexivity.
-Qed.
-
-
-
-
-Inductive cont {G} {rty : type} : type -> Set :=
-| KAppL {L ty1 ty2}
-        (e2 : expr G L ty1)
-        (l : hlist (value G) L)
-        (k : cont ty2)
-        : cont (Arrow ty1 ty2)
-| KAppR {L ty1 ty2}
-        (e1 : expr G L (Arrow ty1 ty2))
-        (l : hlist (value G) L)
-        (k : cont ty2)
-        : cont ty1
-| KConstr {L vtys ety etys ctor ty}
-        (ct : constr_type ctor (vtys ++ [ety] ++ etys) ty)
-        (vs : hlist (expr G L) vtys)
-        (es : hlist (expr G L) etys)
-        (l : hlist (value G) L)
-        (k : cont (ADT ty))
-        : cont ety
-| KClose {L vtys ety etys arg_ty ret_ty}
-        (mb : member (arg_ty, vtys ++ [ety] ++ etys, ret_ty) G)
-        (vs : hlist (expr G L) vtys)
-        (es : hlist (expr G L) etys)
-        (l : hlist (value G) L)
-        (k : cont (Arrow arg_ty ret_ty))
-        : cont ety
-| KElim {L case_tys target_tyn ty}
-        (e : elim case_tys (ADT target_tyn) ty)
-        (cases : hlist (expr G L) case_tys)
-        (l : hlist (value G) L)
-        (k : cont ty)
-        : cont (ADT target_tyn)
-| KStop : cont rty
-.
-Implicit Arguments cont [].
-
-Inductive state {G rty} :=
-| Run {L ty}
-        (e : expr G L ty)
-        (l : hlist (value G) L)
-        (k : cont G rty ty)
-| Stop (v : value G rty).
-Implicit Arguments state [].
-
-Definition run_cont {G rty ty} (k : cont G rty ty) : value G ty -> state G rty :=
-    match k in cont _ _ ty_ return value G ty_ -> state G rty with
-    | KAppL e2 l k => fun v => Run (App (Value v) e2) l k
-    | KAppR e1 l k => fun v => Run (App e1 (Value v)) l k
-    | KConstr ct vs es l k =>
-            fun v => Run (Constr ct (happ vs (hcons (Value v) es))) l k
-    | KClose mb vs es l k =>
-            fun v => Run (Close mb (happ vs (hcons (Value v) es))) l k
-    | KElim e cases l k =>
-            fun v => Run (Elim e cases (Value v)) l k
-    | KStop => fun v => Stop v
-    end.
-
-Definition cont_denote {G rty ty} (g : hlist func_type_denote G) (k : cont G rty ty) :
-        type_denote ty -> type_denote rty :=
-    let locals_denote {tys} (l : hlist _ tys) := value_hlist_denote g l in
-    let fix go {ty} (k : cont G rty ty) :=
-        match k in cont _ _ ty_ return type_denote ty_ -> type_denote rty with
-        | KAppL e2 l k => fun x => go k (x (expr_denote g (locals_denote l) e2))
-        | KAppR e1 l k => fun x => go k ((expr_denote g (locals_denote l) e1) x)
-        | KConstr ct vs es l k => fun x =>
-                let l' := locals_denote l in
-                let vs' := expr_hlist_denote g l' vs in
-                let es' := expr_hlist_denote g l' es in
-                go k (constr_denote ct (happ vs' (hcons x es')))
-        | KClose mb vs es l k => fun x =>
-                let l' := locals_denote l in
-                let vs' := expr_hlist_denote g l' vs in
-                let es' := expr_hlist_denote g l' es in
-                let func := hget g mb in
-                go k (fun arg => func (happ vs' (hcons x es')) arg)
-        | KElim e cases l k => fun x =>
-                let l' := locals_denote l in
-                let cases' := expr_hlist_denote g l' cases in
-                go k (elim_denote e cases' x)
-        | KStop => fun x => x
-        end in go k.
-
-Lemma value_hlist_denote_is_hmap : forall {G} g {tys} vs,
-    @value_hlist_denote G g tys vs = hmap (fun ty v => value_denote g v) vs.
-induction vs; simpl.
-- reflexivity.
-- rewrite IHvs. reflexivity.
-Qed.
-
-Lemma expr_hlist_denote_is_hmap : forall {G L} g l {tys} es,
-    @expr_hlist_denote G L g l tys es = hmap (fun ty e => expr_denote g l e) es.
-induction es; simpl.
-- reflexivity.
-- rewrite IHes. reflexivity.
-Qed.
-
-Definition state_denote {G rty} (g : hlist func_type_denote G) (s : state G rty) :
-        type_denote rty :=
-    match s with
-    | Run e l k =>
-            let e' := expr_denote g (value_hlist_denote g l) e in
-            let k' := cont_denote g k in
-            k' e'
-    | Stop v => value_denote g v
-    end.
-
-
-Definition add_state : state add_G _ :=
-    Run (App (App (Close Here hnil) (Value two)) (Value three)) hnil KStop.
-
-Eval compute in state_denote (genv_denote add_genv) add_state.
-
-
-Inductive sstep {G rty} (g : genv G) : state G rty -> state G rty -> Prop :=
-| SValue : forall {L ty} v (l : hlist (value G) L) (k : cont G rty ty),
-        sstep g (Run (Value v) l k)
-                (run_cont k v)
-
-| SVar : forall {L ty} mb (l : hlist (value G) L) (k : cont G rty ty),
-        sstep g (Run (Var mb) l k)
-                (Run (Value (hget l mb)) l k)
-
-| SAppL : forall {L ty1 ty2} (e1 : expr G L (Arrow ty1 ty2)) (e2 : expr G L ty1) l k,
-        ~ is_value e1 ->
-        sstep g (Run (App e1 e2) l k)
-                (Run e1 l (KAppL e2 l k))
-| SAppR : forall {L ty1 ty2} (e1 : expr G L (Arrow ty1 ty2)) (e2 : expr G L ty1) l k,
-        is_value e1 ->
-        ~ is_value e2 ->
-        sstep g (Run (App e1 e2) l k)
-                (Run e2 l (KAppR e1 l k))
-
-| SMakeCall : forall {L arg_ty free_tys ret_ty}
-            (mb : member (arg_ty, free_tys, ret_ty) G) free arg
-            (l : hlist _ L) k,
-        sstep g (Run (App (Value (VClose mb free)) (Value arg)) l k)
-                (Run (gget_weaken g mb) (hcons arg free) k)
-
-| SConstrStep : forall {L vtys ety etys ctor ty}
-            (ct : constr_type ctor (vtys ++ [ety] ++ etys) ty)
-            (vs : hlist (expr G L) vtys)
-            (e : expr G L ety)
-            (es : hlist (expr G L) etys)
-            (l : hlist _ L) k,
-        HForall (@is_value G L) vs ->
-        ~ is_value e ->
-        sstep g (Run (Constr ct (happ vs (hcons e es))) l k)
-                (Run e l (KConstr ct vs es l k))
-| SConstrDone : forall {L vtys ctor ty}
-            (ct : constr_type ctor vtys ty)
-            (vs : hlist (value G) vtys)
-            (l : hlist _ L) k,
-        let es := hmap (@Value G L) vs in
-        sstep g (Run (Constr ct es) l k)
-                (Run (Value (VConstr ct vs)) l k)
-
-| SCloseStep : forall {L vtys ety etys arg_ty ret_ty}
-            (mb : member (arg_ty, vtys ++ [ety] ++ etys, ret_ty) G)
-            (vs : hlist (expr G L) vtys)
-            (e : expr G L ety)
-            (es : hlist (expr G L) etys)
-            (l : hlist _ L) k,
-        HForall (@is_value G L) vs ->
-        ~ is_value e ->
-        sstep g (Run (Close mb (happ vs (hcons e es))) l k)
-                (Run e l (KClose mb vs es l k))
-| SCloseDone : forall {L vtys arg_ty ret_ty}
-            (mb : member (arg_ty, vtys, ret_ty) G)
-            (vs : hlist (value G) vtys)
-            (l : hlist _ L) k,
-        let es := hmap (@Value G L) vs in
-        sstep g (Run (Close mb es) l k)
-                (Run (Value (VClose mb vs)) l k)
-
-| SElimTarget : forall {L case_tys target_tyn ty}
-            (e : elim case_tys (ADT target_tyn) ty)
-            (cases : hlist (expr G L) case_tys)
-            (target : expr G L (ADT target_tyn))
-            (l : hlist _ L) k,
-        ~ is_value target ->
-        sstep g (Run (Elim e cases target) l k)
-                (Run target l (KElim e cases l k))
-
-| SEliminate : forall {L case_tys target_tyn ty}
-            (e : elim case_tys (ADT target_tyn) ty)
-            (cases : hlist (expr G L) case_tys)
-            (target : value G (ADT target_tyn))
-            (l : hlist _ L) k,
-        sstep g (Run (Elim e cases (Value target)) l k)
-                (Run (run_elim e cases target) l k)
-.
-
-Ltac refold_expr_hlist_denote g l :=
-    fold (@expr_hlist_denote _ _
-        (genv_denote g)
-        (value_hlist_denote (genv_denote g) l)).
-
-Ltac refold_value_hlist_denote g :=
-    fold (@value_hlist_denote _ (genv_denote g)).
-
-Lemma expr_denote_value : forall {G L ty}
-        (g : hlist func_type_denote G)
-        (l : hlist type_denote L)
-        (v : value G ty),
-    expr_denote g l (Value v) = value_denote g v.
-intros. simpl. reflexivity.
-Qed.
-
-Lemma value_denote_htail : forall {G ty tys}
-    (g : hlist func_type_denote G)
-    (vs : hlist (value G) (ty :: tys)),
-    htail (value_hlist_denote g vs) = value_hlist_denote g (htail vs).
-intros.
-pattern vs.
-refine (
-    match vs as vs_ in hlist _ (ty_ :: tys_) return _ vs_ with
-    | hnil => idProp
-    | hcons v vs => _
-    end).
-simpl. reflexivity.
-Qed.
-
-Lemma value_denote_hhead : forall {G ty tys}
-    (g : hlist func_type_denote G)
-    (vs : hlist (value G) (ty :: tys)),
-    hhead (value_hlist_denote g vs) = value_denote g (hhead vs).
-intros.
-pattern vs.
-refine (
-    match vs as vs_ in hlist _ (ty_ :: tys_) return _ vs_ with
-    | hnil => idProp
-    | hcons v vs => _
-    end).
-simpl. reflexivity.
-Qed.
-
-Lemma expr_denote_htail : forall {G L ty tys}
-    (g : hlist func_type_denote G)
-    (l : hlist type_denote L)
-    (es : hlist (expr G L) (ty :: tys)),
-    htail (expr_hlist_denote g l es) = expr_hlist_denote g l (htail es).
-intros.
-pattern es.
-refine (
-    match es as es_ in hlist _ (ty_ :: tys_) return _ es_ with
-    | hnil => idProp
-    | hcons e es => _
-    end).
-simpl. reflexivity.
-Qed.
-
-Lemma expr_denote_hhead : forall {G L ty tys}
-    (g : hlist func_type_denote G)
-    (l : hlist type_denote L)
-    (es : hlist (expr G L) (ty :: tys)),
-    hhead (expr_hlist_denote g l es) = expr_denote g l (hhead es).
-intros.
-pattern es.
-refine (
-    match es as es_ in hlist _ (ty_ :: tys_) return _ es_ with
-    | hnil => idProp
-    | hcons e es => _
-    end).
-simpl. reflexivity.
-Qed.
-
-Hint Rewrite -> @value_denote_htail : hlist_denote_normalize.
-Hint Rewrite -> @value_denote_hhead : hlist_denote_normalize.
-Hint Rewrite -> @expr_denote_htail : hlist_denote_normalize.
-Hint Rewrite -> @expr_denote_hhead : hlist_denote_normalize.
-
-Local Ltac run_elim_refold g l :=
-    fold (@value_hlist_denote _ g);
-    fold (@expr_hlist_denote _ _ g l).
-
-Local Ltac run_elim_solver g l :=
-    simpl; run_elim_refold g l;
-    autorewrite with hlist_denote_normalize; try reflexivity.
-
-Lemma run_elim_denote : forall {G L case_tys target_tyn ret_ty}
-        (g : hlist func_type_denote G)
-        (l : hlist type_denote L)
-        (e : elim case_tys (ADT target_tyn) ret_ty)
-        (cases : hlist (expr G L) case_tys)
-        (target : value G (ADT target_tyn)),
-    elim_denote e (expr_hlist_denote g l cases) (value_denote g target) =
-    expr_denote g l (run_elim e cases target).
-intros.
-
-pattern e.
-refine (
-    match target in value _ (ADT target_tyn_)
-        return forall
-            (e_ : elim case_tys (ADT target_tyn_) ret_ty), _ e_ with
-    | @VConstr _  target_tyn ctor arg_tys  ct args => fun e => _
-    | VClose _ _ => idProp
-    end e).
-clear e0 target target_tyn0.
-
-
-pattern e, cases, ct.
-refine (
-    match e as e_ in elim case_tys_ (ADT target_tyn_) ret_ty_
-        return forall
-            (cases_ : hlist (expr G L) case_tys_)
-            (ct_ : constr_type ctor arg_tys target_tyn_),
-            _ e_ cases_ ct_ with
-    | ENat ret_ty => _
-    | EBool ret_ty => _
-    | EList item_ty ret_ty => _
-    | EUnit ret_ty => _
-    | EPair ty1 ty2 ret_ty => _
-    | EOption item_ty ret_ty => _
-    | EPositive ret_ty => _
-    end cases ct);
-clear e ct target_tyn cases ret_ty0 case_tys; intros cases ct.
-
-- pattern ct, args, cases.
-  refine (
-    match ct as ct_ in constr_type ctor_ arg_tys_ Tnat
-        return forall
-            (args_ : hlist _ arg_tys_)
-            (cases_ : _),
-            _ ct_ args_ cases_ with
-    | CTS => _
-    | CTO => _
-    | _ => idProp
-    end args cases);
-  clear ct cases args arg_tys ctor; intros args cases.
-  all: run_elim_solver g l.
-
-- pattern ct, args, cases.
-  refine (
-    match ct as ct_ in constr_type ctor_ arg_tys_ Tbool
-        return forall
-            (args_ : hlist _ arg_tys_)
-            (cases_ : _),
-            _ ct_ args_ cases_ with
-    | CTtrue => _
-    | CTfalse => _
-    | _ => idProp
-    end args cases);
-  clear ct cases args arg_tys ctor; intros args cases.
-  all: run_elim_solver g l.
-
-- pattern item_ty in cases.
-  pattern item_ty, ct, args, cases.
-  refine (
-    match ct as ct_ in constr_type ctor_ arg_tys_ (Tlist item_ty_)
-        return forall
-            (args_ : hlist _ arg_tys_)
-            (cases_ : _ item_ty_),
-            _ item_ty_ ct_ args_ cases_ with
-    | CTnil item_ty => _
-    | CTcons item_ty => _
-    | _ => idProp
-    end args cases);
-  clear ct cases args arg_tys ctor  item_ty0; intros args cases.
-  all: run_elim_solver g l.
-
-- pattern ct, args, cases.
-  refine (
-    match ct as ct_ in constr_type ctor_ arg_tys_ (Tunit)
-        return forall
-            (args_ : hlist _ arg_tys_)
-            (cases_ : _),
-            _ ct_ args_ cases_ with
-    | CTtt => _
-    | _ => idProp
-    end args cases);
-  clear ct cases args arg_tys ctor; intros args cases.
-  all: run_elim_solver g l.
-
-- pattern ty1, ty2 in cases.
-  pattern ty1, ty2, ct, args, cases.
-  refine (
-    match ct as ct_ in constr_type ctor_ arg_tys_ (Tpair ty1_ ty2_)
-        return forall
-            (args_ : hlist _ arg_tys_)
-            (cases_ : _ ty1_ ty2_),
-            _ ty1_ ty2_ ct_ args_ cases_ with
-    | CTpair ty1 ty2 => _
-    | _ => idProp
-    end args cases);
-  clear ct cases args arg_tys ctor  ty0 ty3; intros args cases.
-  all: run_elim_solver g l.
-
-- pattern item_ty in cases.
-  pattern item_ty, ct, args, cases.
-  refine (
-    match ct as ct_ in constr_type ctor_ arg_tys_ (Toption item_ty_)
-        return forall
-            (args_ : hlist _ arg_tys_)
-            (cases_ : _ item_ty_),
-            _ item_ty_ ct_ args_ cases_ with
-    | CTsome item_ty => _
-    | CTnone item_ty => _
-    | _ => idProp
-    end args cases);
-  clear ct cases args arg_tys ctor  item_ty0; intros args cases.
-  all: run_elim_solver g l.
-
-- pattern ct, args, cases.
-  refine (
-    match ct as ct_ in constr_type ctor_ arg_tys_ (Tpositive)
-        return forall
-            (args_ : hlist _ arg_tys_)
-            (cases_ : _),
-            _ ct_ args_ cases_ with
-    | CTxI => _
-    | CTxO => _
-    | CTxH => _
-    | _ => idProp
-    end args cases);
-  clear ct cases args arg_tys ctor; intros args cases.
-  all: run_elim_solver g l.
-
-Qed.
-
-Theorem sstep_denote : forall {G rty} (g : genv G) (s1 s2 : state G rty),
-    sstep g s1 s2 ->
-    state_denote (genv_denote g) s1 = state_denote (genv_denote g) s2.
-intros0 Hstep. inv Hstep.
-
-- clear Hstep. induction k; simpl; try reflexivity.
-
-  + refold_expr_hlist_denote g l0.
-    do 3 rewrite expr_hlist_denote_is_hmap.
-    rewrite hmap_app. simpl. reflexivity.
-
-  + refold_expr_hlist_denote g l0.
-    do 3 rewrite expr_hlist_denote_is_hmap.
-    rewrite hmap_app. simpl. reflexivity.
-
-- simpl. rewrite value_hlist_denote_is_hmap. rewrite hget_hmap. reflexivity.
-
-- simpl. reflexivity.
-- simpl. reflexivity.
-
-- simpl. fold (@value_hlist_denote _ (genv_denote g)). f_equal.
-  rewrite gget_gget_weaken. eapply genv_denote_gget.
-
-- simpl. refold_expr_hlist_denote g l.
-  do 3 rewrite expr_hlist_denote_is_hmap.
-  rewrite hmap_app. simpl. reflexivity.
-
-- simpl. refold_expr_hlist_denote g l. refold_value_hlist_denote g.
-  unfold es.  rewrite expr_hlist_denote_is_hmap. rewrite hmap_hmap.
-  rewrite value_hlist_denote_is_hmap with (vs0 := vs).
-  simpl. reflexivity.
-
-- simpl. refold_expr_hlist_denote g l.
-  do 3 rewrite expr_hlist_denote_is_hmap.
-  rewrite hmap_app. simpl. reflexivity.
-
-- simpl. refold_expr_hlist_denote g l. refold_value_hlist_denote g.
-  unfold es.  rewrite expr_hlist_denote_is_hmap. rewrite hmap_hmap.
-  rewrite value_hlist_denote_is_hmap with (vs0 := vs).
-  simpl. reflexivity.
-
-- simpl. refold_expr_hlist_denote g l. reflexivity.
-
-- simpl. refold_expr_hlist_denote g l. f_equal.
-  apply run_elim_denote.
-Qed.
