src/SourceLiftedProofs.v
@@ -1,0 +1,568 @@
+Require Import Common.
+
+Require Import FunctionalExtensionality.
+Require Import Program.
+
+Require Import HList.
+
+Require Import Utopia.
+
+Require Import SourceLifted.
+
+
+
+(* induction schemes for value and expr *)
+
+Definition value_rect_mut_comb G
+        (P : forall {ty}, value G ty -> Type)
+        (Pl : forall {tys}, hlist (value G) tys -> Type)
+    (HVConstr : forall {ty ctor arg_tys} (ct : constr_type ctor arg_tys ty) args,
+        Pl args -> P (VConstr ct args))
+    (HVClose : forall {arg_ty free_tys ret_ty} (mb : member (arg_ty, free_tys, ret_ty) G) free,
+        Pl free -> P (VClose mb free))
+    (Hhnil : Pl hnil)
+    (Hhcons : forall {ty tys} (v : value G ty) (vs : hlist (value G) tys),
+        P v -> Pl vs -> Pl (hcons v vs)) :
+    (forall {ty} (v : value G ty), P v) *
+    (forall {tys} (v : hlist (value G) tys), Pl v) :=
+    let fix go {ty} (v : value G ty) :=
+        let fix go_hlist {tys} (vs : hlist (value G) tys) :=
+            match vs as vs_ return Pl vs_ with
+            | hnil => Hhnil
+            | hcons v vs => Hhcons v vs (go v) (go_hlist vs)
+            end in
+        match v as v_ return P v_ with
+        | VConstr ct args => HVConstr ct args (go_hlist args)
+        | VClose mb free => HVClose mb free (go_hlist free)
+        end in
+    let fix go_hlist {tys} (vs : hlist (value G) tys) :=
+        match vs as vs_ return Pl vs_ with
+        | hnil => Hhnil
+        | hcons v vs => Hhcons v vs (go v) (go_hlist vs)
+        end in
+    (@go, @go_hlist).
+
+Definition value_rect_mut G P Pl HVConstr HVClose Hhnil Hhcons :=
+    fst (value_rect_mut_comb G P Pl HVConstr HVClose Hhnil Hhcons).
+
+
+Definition expr_rect_mut_comb G L
+        (P : forall {ty}, expr G L ty -> Type)
+        (Pl : forall {tys}, hlist (expr G L) tys -> Type)
+    (HValue : forall {ty} (v : value G ty), P (Value v))
+    (HVar : forall {ty} (mb : member ty L), P (Var mb))
+    (HApp : forall {ty1 ty2} (f : expr G L (Arrow ty1 ty2)) (a : expr G L ty1),
+        P f -> P a -> P (App f a))
+    (HConstr : forall {ty ctor arg_tys} (ct : constr_type ctor arg_tys ty) args,
+        Pl args -> P (Constr ct args))
+    (HClose : forall {arg_ty free_tys ret_ty} (mb : member (arg_ty, free_tys, ret_ty) G) free,
+        Pl free -> P (Close mb free))
+    (HElim : forall {case_tys target_tyn ty} (e : elim case_tys (ADT target_tyn) ty) cases target,
+        Pl cases -> P target -> P (Elim e cases target))
+    (Hhnil : Pl hnil)
+    (Hhcons : forall {ty tys} (e : expr G L ty) (es : hlist (expr G L) tys),
+        P e -> Pl es -> Pl (hcons e es)) :
+    (forall {ty} (e : expr G L ty), P e) *
+    (forall {tys} (e : hlist (expr G L) tys), Pl e) :=
+    let fix go {ty} (e : expr G L ty) :=
+        let fix go_hlist {tys} (es : hlist (expr G L) tys) :=
+            match es as es_ return Pl es_ with
+            | hnil => Hhnil
+            | hcons e es => Hhcons e es (go e) (go_hlist es)
+            end in
+        match e as e_ return P e_ with
+        | Value v => HValue v
+        | Var mb => HVar mb
+        | App f a => HApp f a (go f) (go a)
+        | Constr ct args => HConstr ct args (go_hlist args)
+        | Close mb free => HClose mb free (go_hlist free)
+        | Elim e cases target => HElim e cases target (go_hlist cases) (go target)
+        end in
+    let fix go_hlist {tys} (es : hlist (expr G L) tys) :=
+        match es as es_ return Pl es_ with
+        | hnil => Hhnil
+        | hcons e es => Hhcons e es (go e) (go_hlist es)
+        end in
+    (@go, @go_hlist).
+
+Definition expr_rect_mut G L P Pl HValue HVar HApp HConstr HClose HElim Hhnil Hhcons :=
+    fst (expr_rect_mut_comb G L P Pl HValue HVar HApp HConstr HClose HElim Hhnil Hhcons).
+
+
+
+(* induction schemes for hlist * member and for glist * member *)
+
+Lemma hlist_member_rect A (B : A -> Type) (ix : A)
+        (P : forall ixs, hlist B ixs -> member ix ixs -> Type)
+    (HHere : forall ixs val vals,
+        P (ix :: ixs) (hcons val vals) Here)
+    (HThere : forall ix' ixs val vals mb
+        (IHmb : P ixs vals mb),
+        P (ix' :: ixs) (hcons val vals) (There mb))
+    : forall ixs vals mb, P ixs vals mb.
+induction vals; intros.
+
+- exfalso.
+  refine (
+    match mb in member _ [] with
+    | Here => idProp
+    | There mb' => idProp
+    end).
+
+- rename a into ix'. rename b into val. rename l into ixs.
+  refine (
+    match mb as mb_ in member _ (ix'_ :: ixs_)
+        return (
+            forall (val_ : B ix'_) (vals_ : hlist B ixs_)
+                (IHvals_ : forall mb, P ixs_ vals_ mb),
+            P (ix'_ :: ixs_) (hcons val_ vals_) mb_) with
+    | Here => _
+    | There mb' => _
+    end val vals IHvals); intros.
+  + eapply HHere.
+  + eapply HThere. eapply IHvals_.
+Defined.
+
+Lemma hlist_member_ind A (B : A -> Type) (ix : A)
+        (P : forall ixs, hlist B ixs -> member ix ixs -> Prop)
+    (HHere : forall ixs val vals,
+        P (ix :: ixs) (hcons val vals) Here)
+    (HThere : forall ix' ixs val vals mb
+        (IHmb : P ixs vals mb),
+        P (ix' :: ixs) (hcons val vals) (There mb))
+    : forall ixs vals mb, P ixs vals mb.
+apply hlist_member_rect; assumption.
+Qed.
+
+
+Lemma genv_member_rect ix
+        (P : forall ixs, genv ixs -> member ix ixs -> Type)
+    (HHere : forall ixs val vals,
+        P (ix :: ixs) (GenvCons val vals) Here)
+    (HThere : forall ix' ixs val vals mb
+        (IHmb : P ixs vals mb),
+        P (ix' :: ixs) (GenvCons val vals) (There mb))
+    : forall G g mb, P G g mb.
+induction g using genv_rect; intros.
+
+- exfalso.
+  refine (
+    match mb in member _ [] with
+    | Here => idProp
+    | There mb' => idProp
+    end).
+
+- rename fn_sig into ix'. rename rest into ixs.
+  rename b into val. rename g into vals.
+  rename IHg into IHvals.
+
+  refine (
+    match mb as mb_ in member _ (ix'_ :: ixs_)
+        return (
+            forall (val_ : body_expr ixs_ ix'_) (vals_ : genv ixs_)
+                (IHvals_ : forall mb, P ixs_ vals_ mb),
+            P (ix'_ :: ixs_) (GenvCons val_ vals_) mb_) with
+    | Here => _
+    | There mb' => _
+    end val vals IHvals); intros.
+
+  + eapply HHere.
+  + eapply HThere. eapply IHvals_.
+Defined.
+
+Lemma genv_member_ind ix
+        (P : forall ixs, genv ixs -> member ix ixs -> Prop)
+    (HHere : forall ixs val vals,
+        P (ix :: ixs) (GenvCons val vals) Here)
+    (HThere : forall ix' ixs val vals mb
+        (IHmb : P ixs vals mb),
+        P (ix' :: ixs) (GenvCons val vals) (There mb))
+    : forall G g mb, P G g mb.
+apply genv_member_rect; assumption.
+Qed.
+
+
+
+(* facts about weakening and denotation *)
+
+Lemma weaken_value_denote : forall {G ty} fn_sig func g (v : value G ty),
+    value_denote g v = value_denote (hcons func g) (weaken_value fn_sig v).
+intros until v.
+induction v using value_rect_mut with
+    (Pl := fun tys vs =>
+        value_hlist_denote g vs =
+        value_hlist_denote _ (weaken_value_hlist fn_sig vs));
+simpl;
+fold (@value_hlist_denote _ g);
+fold (@value_hlist_denote _ (hcons func g));
+fold (@weaken_value_hlist G fn_sig).
+
+- f_equal. exact IHv.
+- rewrite <- IHv. reflexivity.
+
+- reflexivity.
+- erewrite <- IHv, <- IHv0. reflexivity.
+
+Qed.
+
+Lemma weaken_expr_denote : forall {G L ty} fn_sig func g l (e : expr G L ty),
+    expr_denote g l e = expr_denote (hcons func g) l (weaken_expr fn_sig e).
+intros until e.
+induction e using expr_rect_mut with
+    (Pl := fun tys es =>
+        expr_hlist_denote g l es =
+        expr_hlist_denote _ _ (weaken_expr_hlist fn_sig es));
+simpl;
+fold (@expr_hlist_denote _ _ g l);
+fold (@expr_hlist_denote _ _ (hcons func g) l);
+fold (@weaken_expr_hlist G L fn_sig).
+
+- eapply weaken_value_denote.
+- reflexivity.
+- rewrite <- IHe1, <- IHe2. reflexivity.
+- rewrite <- IHe. reflexivity.
+- rewrite <- IHe. reflexivity.
+- rewrite <- IHe, <- IHe0. reflexivity.
+
+- reflexivity.
+- erewrite <- IHe, <- IHe0. reflexivity.
+
+Qed.
+
+Lemma weaken_body_denote : forall {G sig} fn_sig func g (e : body_expr G sig),
+    body_expr_denote g e = body_expr_denote (hcons func g) (weaken_body fn_sig e).
+intros.
+destruct sig as [[? ?] ?]. simpl in *.
+do 2 (eapply functional_extensionality; intro).
+eapply weaken_expr_denote.
+Qed.
+
+
+
+(* facts about genv retrievals.  these are used for the SMakeCall case *)
+
+Lemma genv_denote_gget : forall
+        {G} (g : genv G)
+        {arg_ty free_tys ret_ty} (mb : member (arg_ty, free_tys, ret_ty) G)
+        l x,
+    hget (genv_denote g) mb l x =
+    (let '(e, g') := gget g mb in
+        expr_denote (genv_denote g') (hcons x l) e).
+intros.
+eapply genv_member_ind with (g := g) (mb := mb); intros; simpl.
+- reflexivity.
+- exact IHmb.
+Qed.
+
+Lemma gget_gget_weaken : forall
+        {G} (g : genv G)
+        {arg_ty free_tys ret_ty} (mb : member (arg_ty, free_tys, ret_ty) G)
+        l,
+    expr_denote (genv_denote g) l (gget_weaken g mb) =
+    let '(e, g') := gget g mb in
+        expr_denote (genv_denote g') l e.
+intros.
+eapply genv_member_ind with (g := g) (mb := mb); intros; simpl.
+- rewrite <- weaken_expr_denote. reflexivity.
+- rewrite <- weaken_expr_denote. exact IHmb.
+Qed.
+
+
+
+(* rewrite database for normalizing combinations of hhead/htail and value/expr_denote *)
+
+Lemma value_denote_htail : forall {G ty tys}
+    (g : hlist func_type_denote G)
+    (vs : hlist (value G) (ty :: tys)),
+    htail (value_hlist_denote g vs) = value_hlist_denote g (htail vs).
+intros.
+pattern vs.
+refine (
+    match vs as vs_ in hlist _ (ty_ :: tys_) return _ vs_ with
+    | hnil => idProp
+    | hcons v vs => _
+    end).
+simpl. reflexivity.
+Qed.
+
+Lemma value_denote_hhead : forall {G ty tys}
+    (g : hlist func_type_denote G)
+    (vs : hlist (value G) (ty :: tys)),
+    hhead (value_hlist_denote g vs) = value_denote g (hhead vs).
+intros.
+pattern vs.
+refine (
+    match vs as vs_ in hlist _ (ty_ :: tys_) return _ vs_ with
+    | hnil => idProp
+    | hcons v vs => _
+    end).
+simpl. reflexivity.
+Qed.
+
+Lemma expr_denote_htail : forall {G L ty tys}
+    (g : hlist func_type_denote G)
+    (l : hlist type_denote L)
+    (es : hlist (expr G L) (ty :: tys)),
+    htail (expr_hlist_denote g l es) = expr_hlist_denote g l (htail es).
+intros.
+pattern es.
+refine (
+    match es as es_ in hlist _ (ty_ :: tys_) return _ es_ with
+    | hnil => idProp
+    | hcons e es => _
+    end).
+simpl. reflexivity.
+Qed.
+
+Lemma expr_denote_hhead : forall {G L ty tys}
+    (g : hlist func_type_denote G)
+    (l : hlist type_denote L)
+    (es : hlist (expr G L) (ty :: tys)),
+    hhead (expr_hlist_denote g l es) = expr_denote g l (hhead es).
+intros.
+pattern es.
+refine (
+    match es as es_ in hlist _ (ty_ :: tys_) return _ es_ with
+    | hnil => idProp
+    | hcons e es => _
+    end).
+simpl. reflexivity.
+Qed.
+
+Hint Rewrite -> @value_denote_htail : hlist_denote_normalize.
+Hint Rewrite -> @value_denote_hhead : hlist_denote_normalize.
+Hint Rewrite -> @expr_denote_htail : hlist_denote_normalize.
+Hint Rewrite -> @expr_denote_hhead : hlist_denote_normalize.
+
+
+
+(* run_elim_denote: correspondence between run_elim and elim_denote *)
+
+Local Ltac run_elim_refold g l :=
+    fold (@value_hlist_denote _ g);
+    fold (@expr_hlist_denote _ _ g l).
+
+Local Ltac run_elim_solver g l :=
+    simpl; run_elim_refold g l;
+    autorewrite with hlist_denote_normalize; try reflexivity.
+
+Lemma run_elim_denote : forall {G L case_tys target_tyn ret_ty}
+        (g : hlist func_type_denote G)
+        (l : hlist type_denote L)
+        (e : elim case_tys (ADT target_tyn) ret_ty)
+        (cases : hlist (expr G L) case_tys)
+        (target : value G (ADT target_tyn)),
+    elim_denote e (expr_hlist_denote g l cases) (value_denote g target) =
+    expr_denote g l (run_elim e cases target).
+intros.
+
+pattern e.
+refine (
+    match target in value _ (ADT target_tyn_)
+        return forall
+            (e_ : elim case_tys (ADT target_tyn_) ret_ty), _ e_ with
+    | @VConstr _  target_tyn ctor arg_tys  ct args => fun e => _
+    | VClose _ _ => idProp
+    end e).
+clear e0 target target_tyn0.
+
+
+pattern e, cases, ct.
+refine (
+    match e as e_ in elim case_tys_ (ADT target_tyn_) ret_ty_
+        return forall
+            (cases_ : hlist (expr G L) case_tys_)
+            (ct_ : constr_type ctor arg_tys target_tyn_),
+            _ e_ cases_ ct_ with
+    | ENat ret_ty => _
+    | EBool ret_ty => _
+    | EList item_ty ret_ty => _
+    | EUnit ret_ty => _
+    | EPair ty1 ty2 ret_ty => _
+    | EOption item_ty ret_ty => _
+    | EPositive ret_ty => _
+    end cases ct);
+clear e ct target_tyn cases ret_ty0 case_tys; intros cases ct.
+
+- pattern ct, args, cases.
+  refine (
+    match ct as ct_ in constr_type ctor_ arg_tys_ Tnat
+        return forall
+            (args_ : hlist _ arg_tys_)
+            (cases_ : _),
+            _ ct_ args_ cases_ with
+    | CTS => _
+    | CTO => _
+    | _ => idProp
+    end args cases);
+  clear ct cases args arg_tys ctor; intros args cases.
+  all: run_elim_solver g l.
+
+- pattern ct, args, cases.
+  refine (
+    match ct as ct_ in constr_type ctor_ arg_tys_ Tbool
+        return forall
+            (args_ : hlist _ arg_tys_)
+            (cases_ : _),
+            _ ct_ args_ cases_ with
+    | CTtrue => _
+    | CTfalse => _
+    | _ => idProp
+    end args cases);
+  clear ct cases args arg_tys ctor; intros args cases.
+  all: run_elim_solver g l.
+
+- pattern item_ty in cases.
+  pattern item_ty, ct, args, cases.
+  refine (
+    match ct as ct_ in constr_type ctor_ arg_tys_ (Tlist item_ty_)
+        return forall
+            (args_ : hlist _ arg_tys_)
+            (cases_ : _ item_ty_),
+            _ item_ty_ ct_ args_ cases_ with
+    | CTnil item_ty => _
+    | CTcons item_ty => _
+    | _ => idProp
+    end args cases);
+  clear ct cases args arg_tys ctor  item_ty0; intros args cases.
+  all: run_elim_solver g l.
+
+- pattern ct, args, cases.
+  refine (
+    match ct as ct_ in constr_type ctor_ arg_tys_ (Tunit)
+        return forall
+            (args_ : hlist _ arg_tys_)
+            (cases_ : _),
+            _ ct_ args_ cases_ with
+    | CTtt => _
+    | _ => idProp
+    end args cases);
+  clear ct cases args arg_tys ctor; intros args cases.
+  all: run_elim_solver g l.
+
+- pattern ty1, ty2 in cases.
+  pattern ty1, ty2, ct, args, cases.
+  refine (
+    match ct as ct_ in constr_type ctor_ arg_tys_ (Tpair ty1_ ty2_)
+        return forall
+            (args_ : hlist _ arg_tys_)
+            (cases_ : _ ty1_ ty2_),
+            _ ty1_ ty2_ ct_ args_ cases_ with
+    | CTpair ty1 ty2 => _
+    | _ => idProp
+    end args cases);
+  clear ct cases args arg_tys ctor  ty0 ty3; intros args cases.
+  all: run_elim_solver g l.
+
+- pattern item_ty in cases.
+  pattern item_ty, ct, args, cases.
+  refine (
+    match ct as ct_ in constr_type ctor_ arg_tys_ (Toption item_ty_)
+        return forall
+            (args_ : hlist _ arg_tys_)
+            (cases_ : _ item_ty_),
+            _ item_ty_ ct_ args_ cases_ with
+    | CTsome item_ty => _
+    | CTnone item_ty => _
+    | _ => idProp
+    end args cases);
+  clear ct cases args arg_tys ctor  item_ty0; intros args cases.
+  all: run_elim_solver g l.
+
+- pattern ct, args, cases.
+  refine (
+    match ct as ct_ in constr_type ctor_ arg_tys_ (Tpositive)
+        return forall
+            (args_ : hlist _ arg_tys_)
+            (cases_ : _),
+            _ ct_ args_ cases_ with
+    | CTxI => _
+    | CTxO => _
+    | CTxH => _
+    | _ => idProp
+    end args cases);
+  clear ct cases args arg_tys ctor; intros args cases.
+  all: run_elim_solver g l.
+
+Qed.
+
+
+
+(* misc. helpers for sstep_denote *)
+
+Lemma value_hlist_denote_is_hmap : forall {G} g {tys} vs,
+    @value_hlist_denote G g tys vs = hmap (fun ty v => value_denote g v) vs.
+induction vs; simpl.
+- reflexivity.
+- rewrite IHvs. reflexivity.
+Qed.
+
+Lemma expr_hlist_denote_is_hmap : forall {G L} g l {tys} es,
+    @expr_hlist_denote G L g l tys es = hmap (fun ty e => expr_denote g l e) es.
+induction es; simpl.
+- reflexivity.
+- rewrite IHes. reflexivity.
+Qed.
+
+Ltac refold_expr_hlist_denote g l :=
+    fold (@expr_hlist_denote _ _
+        (genv_denote g)
+        (value_hlist_denote (genv_denote g) l)).
+
+Ltac refold_value_hlist_denote g :=
+    fold (@value_hlist_denote _ (genv_denote g)).
+
+
+
+(* the main theorem: denotation is preserved when taking a step *)
+
+Theorem sstep_denote : forall {G rty} (g : genv G) (s1 s2 : state G rty),
+    sstep g s1 s2 ->
+    state_denote (genv_denote g) s1 = state_denote (genv_denote g) s2.
+intros0 Hstep. inv Hstep.
+
+- clear Hstep. induction k; simpl; try reflexivity.
+
+  + refold_expr_hlist_denote g l0.
+    do 3 rewrite expr_hlist_denote_is_hmap.
+    rewrite hmap_app. simpl. reflexivity.
+
+  + refold_expr_hlist_denote g l0.
+    do 3 rewrite expr_hlist_denote_is_hmap.
+    rewrite hmap_app. simpl. reflexivity.
+
+- simpl. rewrite value_hlist_denote_is_hmap. rewrite hget_hmap. reflexivity.
+
+- simpl. reflexivity.
+- simpl. reflexivity.
+
+- simpl. fold (@value_hlist_denote _ (genv_denote g)). f_equal.
+  rewrite gget_gget_weaken. eapply genv_denote_gget.
+
+- simpl. refold_expr_hlist_denote g l.
+  do 3 rewrite expr_hlist_denote_is_hmap.
+  rewrite hmap_app. simpl. reflexivity.
+
+- simpl. refold_expr_hlist_denote g l. refold_value_hlist_denote g.
+  unfold es.  rewrite expr_hlist_denote_is_hmap. rewrite hmap_hmap.
+  rewrite value_hlist_denote_is_hmap with (vs0 := vs).
+  simpl. reflexivity.
+
+- simpl. refold_expr_hlist_denote g l.
+  do 3 rewrite expr_hlist_denote_is_hmap.
+  rewrite hmap_app. simpl. reflexivity.
+
+- simpl. refold_expr_hlist_denote g l. refold_value_hlist_denote g.
+  unfold es.  rewrite expr_hlist_denote_is_hmap. rewrite hmap_hmap.
+  rewrite value_hlist_denote_is_hmap with (vs0 := vs).
+  simpl. reflexivity.
+
+- simpl. refold_expr_hlist_denote g l. reflexivity.
+
+- simpl. refold_expr_hlist_denote g l. f_equal.
+  apply run_elim_denote.
+Qed.
+
+
+
+
